

Número: 1.1.4.

Ubicación: Pág. 4. Sección 1.1.

Texto:

(Cat2) Si $f, g, h \in \vec{\mathcal{C}}$, tales que

$$\text{cod}(f) = \text{dom}(g) , \text{cod}(g) = \text{dom}(h),$$

entonces $h \circ (g \circ f) = (h \circ g) \circ f$.

(Cat3) Si $f, g \in \vec{\mathcal{C}}$, son tales que $\text{cod}(f) = \text{dom}(g)$, entonces

$$\text{dom}(g \circ f) = \text{dom}(f).$$

(Cat4) Si $f, g \in \vec{\mathcal{C}}$, son tales que $\text{cod}(f) = \text{dom}(g)$, entonces

$$\text{cod}(g \circ f) = \text{cod}(g).$$

Explicación: Se requiere saber primero que si

$$\text{cod}(g) = \text{dom}(h),$$

entonces

$$\text{cod}(g \circ f) = \text{dom}(h).$$

Para componer los 3 morfismos en **(Cat2)**.

Sugerencia:

(Cat2) Si $f, g \in \vec{\mathcal{C}}$, son tales que $\text{cod}(f) = \text{dom}(g)$, entonces $\text{dom}(g \circ f) = \text{dom}(f)$.

(Cat3) Si $f, g \in \vec{\mathcal{C}}$, son tales que $\text{cod}(f) = \text{dom}(g)$, entonces $\text{cod}(g \circ f) = \text{cod}(g)$.

(Cat4) Si $f, g, h \in \vec{\mathcal{C}}$, tales que

$$\text{cod}(f) = \text{dom}(g), \text{cod}(g) = \text{dom}(h),$$

$$\text{entonces } h \circ (g \circ f) = (h \circ g) \circ f.$$